Playground.v
@@ -5,6 +5,7 @@ Require Import RAC.Semantics.
 Require Import ZArith.ZArith.
 Require Import String.
 From Coq Require Import Lists.List.
+From Coq Require Import Logic.FunctionalExtensionality.
 Open Scope string_scope.
 Open Scope Z_scope.
 
@@ -17,14 +18,13 @@ Fact ir5 : Int.inRange 5. now split. Qed.
 Fact ir10 : Int.inRange 10 . now split. Qed.
 Fact ir14 : Int.inRange 14. now split. Qed.
 Fact ir15 : Int.inRange 15. now split. Qed.
-Definition zero := Int.of_z 0 zeroinRange.
-Definition three := Int.of_z 3 ir3.
-Definition five := Int.of_z 5 ir5.
-Definition ten := Int.of_z 10 ir10.
-Definition fifteen := Int.of_z 15 ir15.
+Definition three := Int (Int.of_z 3 ir3).
+Definition five := Int (Int.of_z 5 ir5).
+Definition ten := Int (Int.of_z 10 ir10).
+Definition fifteen := Int (Int.of_z 15 ir15).
 
 
-Example imptest :
+Example stmt_test :
     forall o m,     
     let v := fst o in 
     let l := snd o in 
@@ -44,18 +44,18 @@ Example imptest :
 
    }>
     
-    (v{"x" \ five}{"y"\ten}{"z"\fifteen}{"g"\zero}{"g"\three}, l) m
+    (v{"g"\ three, "g"\ zero, "z"\ fifteen, "y"\ ten, "x" \ five}, l) m
    .
 Proof.
     intros.
      apply S_Seq with (v{"x" \ five},l) m.
      apply S_Assign. apply C_E_Int.
-     apply S_Seq with (v{"x" \ five}{"y" \ ten}, l) m.
+     apply S_Seq with (v{"y"\ten,"x"\five}, l) m.
      - apply S_Assign. apply C_E_Int.
-     - apply S_Seq with (v{"x" \ five}{"y" \ ten}{"z" \ fifteen}, l) m.
+     - apply S_Seq with (v{"z" \ fifteen, "y" \ ten, "x" \ five}, l) m.
         + apply S_Assign. apply C_E_BinOpInt with (z:=5) (z':=10) (z_ir:=ir5) (z'_ir:=ir10) ; 
           now apply C_E_Var. 
-        + apply S_Seq  with (v{"x" \ five}{"y" \ ten}{"z" \ fifteen}{"g"\ zero}, l) m. 
+        + apply S_Seq  with (v{"g"\ zero, "z" \ fifteen, "y" \ ten, "x" \ five}, l) m. 
           ++ apply S_Assign. apply C_E_Int.
           ++ apply S_IfFalse with zero.
             * apply C_E_BinOpFalse with 15 14 ir15 ir14 ; try now constructor.
@@ -63,6 +63,7 @@ Proof.
             * reflexivity.
             * apply S_Assign. apply C_E_BinOpInt with  (z:=15) (z':=5) (z_ir:=ir15) (z'_ir:=ir5); now constructor.
 Qed.
+
 
 Close Scope mini_c_scope.
 
